Greta.lean
@@ -8,8 +8,11 @@ import Greta.Examples
 import Greta.Learn
 import Greta.GenTA
 import Greta.Intersect
+import Greta.IntersectSpec
 import Greta.Soundness
 import Greta.GenTASpec
+import Greta.LearnSpec
+import Greta.RefLearn
 import Greta.Serialize
 import Greta.Enumerate
 import Greta.Test
